Lang: add `extended` core with DecidableEq and OfNat

Clap/Sha2Test.lean
@@ -2,7 +2,7 @@ import Clap.Sha2Circuit
 import Clap.Sha2Cpu
 import Clap.Sha2
 
-namespace TestUInt
+namespace TestCpu
 
 open Clap.Sha2
 
@@ -11,31 +11,32 @@ def stringToU8s (s:String) : Array UInt8 :=
   let bs : Array UInt8 := bs.data
   bs
 
-#guard digest (t := Clap.Sha2.Cpu.t) (stringToU8s "abc") =
-  #[0xba7816bf, 0x8f01cfea, 0x414140de, 0x5dae2223, 0xb00361a3, 0x96177a9c, 0xb410ff61, 0xf20015ad]
+example : digest (t := Clap.Sha2.Cpu.t) (stringToU8s "abc") =
+  #[0xba7816bf, 0x8f01cfea, 0x414140de, 0x5dae2223, 0xb00361a3, 0x96177a9c, 0xb410ff61, 0xf20015ad] := by
+  native_decide
 
-#guard digest (t := Clap.Sha2.Cpu.t) (stringToU8s "abcdbcdecdefdefgefghfghighijhijkijkljklmklmnlmnomnopnopq") =
-  #[0x248d6a61, 0xd20638b8, 0xe5c02693, 0x0c3e6039, 0xa33ce459, 0x64ff2167, 0xf6ecedd4, 0x19db06c1]
+example : digest (t := Clap.Sha2.Cpu.t) (stringToU8s "abcdbcdecdefdefgefghfghighijhijkijkljklmklmnlmnomnopnopq") =
+  #[0x248d6a61, 0xd20638b8, 0xe5c02693, 0x0c3e6039, 0xa33ce459, 0x64ff2167, 0xf6ecedd4, 0x19db06c1] := by
+  native_decide
 
-end TestUInt
+end TestCpu
 
 namespace TestCircuit
 
-open Clap.Sha2
-open Clap.Lang
-
 abbrev p := Primes.goldilocks
-abbrev F' := ZMod p
+
+open Clap.Sha2
+open Clap.Lang Core ZMod
 
 def stringToU8s (s:String) : Array (F8 p) :=
   let bs : ByteArray := s.toUTF8
   let bs : Array UInt8 := bs.data
   bs.map fun b =>
-    let b : F' := (b.toNat : F')
+    let b : F p := (b.toNat : F p)
     F8.ofF b
 
 def testDigest (s : String) (expected : Array UInt32) : Option Unit := do
-  let expected := expected.map fun u32 => F32.ofF (u32.toNat: F')
+  let expected := expected.map fun u32 => F32.ofF (u32.toNat: F p)
   let d := digest (t := Clap.Sha2.Circuit.t p) (stringToU8s s)
   for (d,e) in d.zip expected do
     F8.assert_eq d e
