Clap/Sha2Circuit.lean
@@ -7,7 +7,7 @@ namespace Clap.Sha2.Circuit
 
 open Clap.Lang
 
-variable {p : ℕ} [Fact (Nat.Prime p)] [Core p] [Fact (Primes.fits p 8)] [Fact (Primes.fits p 32)]
+variable {p : ℕ} [Core p] [Fact (Primes.fits p 8)] [Fact (Primes.fits p 32)]
 
 open Core
 
@@ -74,7 +74,7 @@ def shiftRight (n : USize) (x : F32 p) : F32 p :=
   let l := List.drop n.toNat x
   l ++ List.replicate n.toNat 0
 
-abbrev t p [Fact (Nat.Prime p)] [Core p] [Fact (Primes.fits p 8)] [Fact (Primes.fits p 32)] : Clap.Sha2.T := {
+abbrev t p [Core p] [Fact (Primes.fits p 8)] [Fact (Primes.fits p 32)] : Clap.Sha2.T := {
   US:=F (p:=p),
   U8:=F8 (p:=p),
   U32:=F32 (p:=p)
@@ -107,10 +107,9 @@ end Clap.Sha2.Circuit
 namespace Tests
 
 abbrev p := Primes.goldilocks
-abbrev F := ZMod p
 
-open Clap.Lang
 open Clap.Sha2.Circuit
+open Clap.Lang Core ZMod
 
 instance : Coe ℕ (List (ZMod p)) where
   coe n := Clap.num2bitsLsbPure (p:=p) 32 (n:ZMod p)
